Add scratch work

src/Typing.v
@@ -2,6 +2,8 @@ From TLC Require Import LibString LibList LibSet LibMap.
 From MCore Require Import Syntax Ctx Tactics.
 Import LibListNotation.
 
+Open Scope liblist_scope.
+
 Module Typing (P : PAT).
   Module C := Ctx P.
   Export C.
@@ -22,10 +24,10 @@ Module Typing (P : PAT).
 
     Definition ok_data (Gamma : ctx) (d : data) : Prop :=
       forall T cons,
-        d[T] = cons ->
-        tname_in T Gamma /\
+        binds d T cons ->
+        in_ctx T BindTName Gamma /\
           forall K,
-            K \in (cons : set con) -> exists d ty, con_in K d ty T Gamma
+            K \in cons -> exists d ty, in_ctx K (BindCon d ty T) Gamma
     .
 
     Inductive ok_kind : ctx -> kind -> Prop :=
@@ -42,15 +44,16 @@ Module Typing (P : PAT).
     Inductive ok_type : ctx -> type -> kind -> Prop :=
     | KVar : forall Gamma tv k,
         ok_ctx Gamma ->
-        tvar_in tv k Gamma ->
+        in_ctx tv (BindTVar k) Gamma ->
         Gamma |= TyFVar tv ~:: k
     | KArr : forall Gamma ty1 ty2,
         Gamma |= ty1 ~:: KiType ->
         Gamma |= ty2 ~:: KiType ->
         Gamma |= TyArr ty1 ty2 ~:: KiType
-    | KAll : forall Gamma k ty,
+    | KAll : forall X Gamma k ty,
+        X = length Gamma ->
         ok_kind Gamma k ->
-        Gamma & BindTVar k |= {0 ~> TyFVar (length Gamma)} ty ~:: KiType ->
+        Gamma & BindTVar k |= {0 ~> TyFVar X} ty ~:: KiType ->
         Gamma |= TyAll k ty ~:: KiType
     (* | TyProd' : forall {Gamma : ctx} {ty1 ty2 : type}, *)
     (*     ok_type Gamma ty1 KiType -> *)
@@ -82,7 +85,7 @@ Module Typing (P : PAT).
         ok_ctx Gamma ->
         ok_data Gamma d ->
         Gamma |= ty ~:: KiType ->
-        tname_in T Gamma ->
+        in_ctx T BindTName Gamma ->
         ok_ctx (Gamma & BindCon d ty T)
     | CtxTVar : forall Gamma k,
         ok_ctx Gamma ->
@@ -92,9 +95,12 @@ Module Typing (P : PAT).
         ok_ctx Gamma ->
         Gamma |= ty ~:: KiType ->
         ok_ctx (Gamma & BindVar ty)
-    | CtxMatch : forall Gamma m,
+    | CtxSkip : forall Gamma,
         ok_ctx Gamma ->
-        ok_ctx (Gamma & BindMatch m)
+        ok_ctx (Gamma & Skip)
+    (* | CtxMatch : forall Gamma m, *)
+    (*     ok_ctx Gamma -> *)
+    (*     ok_ctx (Gamma & BindMatch m) *)
     .
     #[export]
      Hint Constructors ok_type : mcore.
@@ -105,21 +111,23 @@ Module Typing (P : PAT).
     Inductive ok_term : ctx -> term -> type -> Prop :=
     | TVar : forall Gamma x ty,
         ok_ctx Gamma ->
-        binds x (BindVar ty) Gamma ->
+        in_ctx x (BindVar ty) Gamma ->
         Gamma |= TmFVar x ~: ty
-    | TLam : forall L Gamma ty1 ty2 t,
+    | TLam : forall x Gamma ty1 ty2 t,
+        x = length Gamma ->
+        fresh x t ->
         Gamma |= ty1 ~:: KiType ->
-        (forall x, x \notin L ->
-                   (Gamma & x ~ BindVar ty1) |= [0 ~> TmFVar x]t ~: ty2) ->
+        Gamma & BindVar ty1 |= [0 ~> TmFVar x]t ~: ty2 ->
         Gamma |= TmLam ty1 t ~: TyArr ty1 ty2
     | TApp : forall Gamma ty1 ty2 t1 t2,
         Gamma |= t1 ~: TyArr ty1 ty2 ->
         Gamma |= t2 ~: ty1 ->
         Gamma |= TmApp t1 t2 ~: ty2
-    | TTyLam : forall L Gamma k ty t,
+    | TTyLam : forall X Gamma k ty t,
+        X = length Gamma ->
+        tfresh_t X t -> tfresh X ty ->
         ok_kind Gamma k ->
-        (forall X, X \notin L ->
-                   (Gamma & X ~ BindTVar k) |= [{0 ~> TyFVar X}]t ~: ({0 ~> TyFVar X}ty)) ->
+        Gamma & BindTVar k |= [{0 ~> TyFVar X}]t ~: ({0 ~> TyFVar X}ty) ->
         Gamma |= TmTyLam k t ~: (TyAll k ty)
     | TTyApp : forall Gamma k ty1 ty2 t,
         Gamma |= t ~: TyAll k ty1 ->
@@ -205,430 +213,475 @@ Module Typing (P : PAT).
     (** PROPERTIES OF TYPING **)
     (**************************)
 
-    Lemma ok_ctx_ok :
-      forall Gamma,
-        ok_ctx Gamma ->
-        ok Gamma.
-    Proof. introv Hctx ; induction* Hctx. Qed.
-    #[export]
-     Hint Resolve ok_ctx_ok : mcore.
-
-    Lemma ok_kind_weakening :
-      forall G3 G1 G2 k,
-        ok_kind (G1 & G3) k ->
-        ok_kind (G1 & G2 & G3) k.
-    Proof. introv Hk. induction* Hk. Qed.
-
-    Lemma ok_type_weakening :
-      forall G3 G1 G2 T k,
-        G1 & G3 |= T ~:: k ->
-        ok_ctx (G1 & G2 & G3) ->
-        G1 & G2 & G3 |= T ~:: k.
-    Proof.
-      introv Hk Hctx.
-      remember (G1 & G3) as Gamma. gen G3.
-      induction* Hk; intros; substs.
-      { Case "TyFVar". constructors*. apply* binds_weaken. }
-      { Case "TyAll". apply_fresh* KAll. apply* ok_kind_weakening.
-        apply_ih_bind* H1.
-        constructor*. apply* ok_kind_weakening. }
-    Qed.
-
-    Lemma ok_ctx_ok_type :
-      forall Gamma x T,
-        ok_ctx Gamma ->
-        binds x (BindVar T) Gamma ->
-        Gamma |= T ~:: KiType.
-    Proof.
-      introv Hctx Hbind.
-      induction* Hctx ; try (binds_cases Hbind ; apply_empty* ok_type_weakening).
-      { Case "CtxEmpty". false. apply* binds_empty_inv. }
-      { Case "CtxVar". inverts* EQ. }
-    Qed.
-
-    Lemma ok_type_lct :
-      forall Gamma T k,
-        Gamma |= T ~:: k ->
-        lct T.
-    Proof. introv Hk ; induction* Hk. Qed.
-    #[export]
-     Hint Resolve ok_type_lct : mcore.
-
-    Lemma ok_term_lct :
-      forall Gamma t T,
-        Gamma |= t ~: T ->
-        lct T.
-    Proof with eauto using ok_ctx_ok_type, ok_type_lct.
-      introv hasType.
-      induction* hasType...
-      { Case "TmLam". constructors...
-        pick_fresh_gen L y... }
-      { Case "TmApp". inverts* IHhasType1. }
-      { Case "TmTyLam". inverts* IHhasType.
-        assert(Hlct: lct ty2)...
-        pick_fresh X. rewrite *(@tsubst_intro X).
-        apply* tsubst_lct. }
-    Qed.
-    #[export]
-     Hint Resolve ok_term_lct : mcore.
-
-    Lemma ok_term_lc :
-      forall Gamma t T,
-        Gamma |= t ~: T ->
-        lc t.
-    Proof with eauto using ok_term_lct, ok_type_lct with mcore.
-      introv Htype.
-      induction* Htype; intros.
-    Qed.
-    #[export]
-     Hint Resolve ok_term_lc : mcore.
-
-    Lemma ok_ctx_push :
-      forall G1 x b,
-        ok_ctx (G1 & x ~ b) ->
-        ok_ctx G1.
-    Proof.
-      introv Hwf.
-      inverts Hwf ; try (apply eq_push_inv in H; inverts H as []; substs*).
-      false. apply *empty_push_inv.
-    Qed.
-
-    Lemma ok_type_ok_ctx :
-      forall Gamma T k,
-        Gamma |= T ~:: k ->
-        ok_ctx Gamma.
-    Proof.
-      introv hasType.
-      induction* hasType; pick_fresh_gen L x;
-        eauto using ok_ctx_push.
-    Qed.
-    #[export]
-     Hint Resolve ok_type_ok_ctx : mcore.
-
-    Lemma ok_term_ok_ctx :
-      forall Gamma t T,
-        Gamma |= t ~: T ->
-        ok_ctx Gamma.
-    Proof.
-      introv hasType.
-      induction* hasType; pick_fresh_gen L x;
-        eauto using ok_ctx_push.
-    Qed.
-    #[export]
-     Hint Resolve ok_term_ok_ctx : mcore.
-
     Lemma ok_term_weakening :
-      forall G3 G2 G1 t T,
-        G1 & G3 |= t ~: T ->
-        ok_ctx (G1 & G2 & G3) ->
-        G1 & G2 & G3 |= t ~: T.
+      forall x b G1 G2 T1 t1,
+        x = length G1 ->
+        G1 ++ G2 |= t1 ~: T1 ->
+        G1 & b ++ map (bshift x) G2 |= shift x t1 ~: tshift x T1.
     Proof.
-      introv hasType Hctx. remember (G1 & G3) as H. gen G3.
-      induction hasType; intros; substs*.
-      { Case "TmFVar". constructors*. apply* binds_weaken. }
-      { Case "TmLam". apply_fresh* TLam as y.
-        - apply* ok_type_weakening.
-        - apply_ih_bind* H1.
-          constructors*.
-          apply* ok_type_weakening. }
-      { Case "TmTyLam". apply_fresh* TTyLam as X.
-        - apply* ok_kind_weakening.
-        - apply_ih_bind* H1. constructors*. apply* ok_kind_weakening. }
-      { Case "TmTyApp". constructors*. apply* ok_type_weakening. }
-    Qed.
-
-    Lemma ok_data_strengthening :
-      forall G1 G2 x T d,
-        ok_data (G1 & x ~ BindVar T & G2) d ->
-        ok_data (G1 & G2) d.
-    Proof.
-      introv Hd. unfolds ok_data.
-      splits*. introv Hbind.
-      lets [Hbind' Hk]: (proj2 Hd) Hbind.
-      splits.
-      - binds_cases Hbind' ; auto.
-      - introv Hkin. lets [ ? (? & Hbindk) ] : Hk Hkin.
-        binds_cases Hbindk ; eauto.
-    Qed.
-
-    Lemma ok_kind_strengthening :
-      forall G1 G2 x T k,
-        ok_kind (G1 & x ~ BindVar T & G2) k ->
-        ok_kind (G1 & G2) k.
-    Proof. introv Hk. induction* Hk. Qed.
-
-    Lemma ok_type_strengthening :
-      forall G1 G2 x T1 T2 k,
-        G1 & x ~ BindVar T2 & G2 |= T1 ~:: k ->
-        ok_ctx (G1 & G2) ->
-        G1 & G2 |= T1 ~:: k.
-    Proof.
-      introv Htk. remember (G1 & x ~ BindVar T2 & G2) as G. gen G2.
-      induction Htk; intros; substs*.
-      { Case "TyFVar". constructors*.
-        binds_cases H0 ; auto. }
-      { Case "TyAll". apply_fresh* KAll as X.
-        apply* ok_kind_strengthening.
-        apply_ih_bind* H1. constructor*. apply* ok_kind_strengthening. }
-    Qed.
-
-    Lemma ok_ctx_con_inv :
-      forall Gamma K d ty T,
-        ok_ctx (Gamma & K ~ BindCon d ty T) ->
-        ok_data Gamma d /\ Gamma |= ty ~:: KiType /\ binds T BindTName Gamma.
-    Proof.
-      introv Hctx.
-      inverts Hctx ; try (apply eq_push_inv in H as (? & ? & ?); substs* ; splits* ; fequals).
-      false. apply* empty_push_inv.
-    Qed.
-
-    Lemma ok_ctx_tvar_inv :
-      forall Gamma X k,
-        ok_ctx (Gamma & X ~ BindTVar k) ->
-        ok_kind Gamma k.
-    Proof.
-      introv Hctx.
-      inverts Hctx ; try (apply eq_push_inv in H as (? & ? & ?); substs* ; fequals).
-      false. apply* empty_push_inv.
-    Qed.
-
-    Lemma ok_ctx_var_inv :
-      forall Gamma x T,
-        ok_ctx (Gamma & x ~ BindVar T) ->
-        Gamma |= T ~:: KiType.
-    Proof.
-      introv Hctx.
-      inverts Hctx ; try (apply eq_push_inv in H as (? & ? & ?); substs* ; fequals).
-      false. apply* empty_push_inv.
-    Qed.
-
-    Lemma ok_ctx_strengthening :
-      forall G1 x T G3,
-        ok_ctx (G1 & x ~ BindVar T & G3) ->
-        ok_ctx (G1 & G3).
-    Proof.
-      introv Hctx. induction G3 using ctx_ind.
-      { Case "Empty". rewrite concat_empty_r in *. apply* ok_ctx_push. }
-      { Case "Push". rewrite concat_assoc in *.
-        specializes IHG3 (ok_ctx_push _ _ _ Hctx).
-        lets [? Hdisj] : ok_push_inv (ok_ctx_ok _ Hctx).
-        destruct v.
-        { SCase "BindTName". constructor~. }
-        { SCase "BindCon". forwards [ Hd (Htk & HT)]: ok_ctx_con_inv Hctx.
-          constructor~.
-          - applys ok_data_strengthening Hd.
-          - applys* ok_type_strengthening Htk.
-          - binds_cases HT ; auto. }
-        { SCase "BindTVar". forwards Hk: ok_ctx_tvar_inv Hctx.
-          constructor~. applys ok_kind_strengthening Hk. }
-        { SCase "BindVar". forwards Htk: ok_ctx_var_inv Hctx.
-          constructor~. applys* ok_type_strengthening Htk. }
-        { SCase "BindMatch". constructor~. } }
-    Qed.
+      introv hasType.
+      induction hasType ; simple_math.
+      - constructor*. admit.
+      - apply (TLam (S x)). rew_list*. admit. admit. apply* ok_term_subst_comm.
+      - apply (TTyLam (S X)). rew_list*. admit. admit. admit. apply* ok_term_tsubst_comm.
+      - constructors*. admit.
+    Admitted.
 
     Lemma ok_term_subst :
       forall G2 G1 x T1 T2 t1 t2,
-        G1 & x ~ BindVar T2 & G2 |= t1 ~: T1 ->
-        G1 |= t2 ~: T2 ->
-        G1 & G2 |= [x => t2]t1 ~: T1.
-    Proof with eauto using ok_term_lc, ok_ctx_strengthening, ok_type_strengthening with mcore.
-      introv hasType1 hasType2.
-      remember (G1 & x ~ BindVar T2 & G2) as G. gen G2.
+        x = length G1 ->
+        (G1 & BindVar T2 ++ G2) |= t1 ~: T1 ->
+        (G1 & Skip ++ G2) |= t2 ~: T2 ->
+        (G1 & Skip ++ G2) |= [x => t2]t1 ~: T1.
+    Proof.
+      introv Heq hasType1 hasType2.
+      remember (G1 & BindVar T2 ++ G2) as G. gen G2.
       induction hasType1; intros; simpls; substs...
-      { Case "TmFVar". solve_var.
-        - binds_get H0... apply_empty ok_term_weakening...
-        - binds_cases H0... }
-      { Case "TmLam". apply_fresh* TLam as y...
-        rewrite subst_open_comm... apply_ih_bind* H1. }
-      { Case "TmTyLam". apply_fresh* TTyLam as X. apply* ok_kind_strengthening.
-        rewrite* topen_t_subst_comm. apply_ih_bind* H1. }
-      { Case "TmTyApp". constructors*. apply* ok_type_strengthening. }
-    Qed.
+      { Case "TmFVar". simple_math. admit. admit. }
+      { Case "TmLam". apply* (TLam (length (G1 & Skip ++ G2))). admit.
+        rewrite subst_open_comm.
+        replaces (length (G1 & Skip ++ G2)) with (length (G1 & BindVar T2 ++ G2)).
+        rew_list. simple_math. rew_list in *.
+        applys_eq (>> IHhasType1 (G2 & BindVar ty1)).
+        rew_list*. rew_list*. admit. rew_list*. simple_math. admit.
+        rewrite H.
+        (* rewrite subst_open_comm... apply_ih_bind* H1. } *)
+    (*   { Case "TmTyLam". apply_fresh* TTyLam as X. apply* ok_kind_strengthening. *)
+    (*     rewrite* topen_t_subst_comm. apply_ih_bind* H1. } *)
+    (*   { Case "TmTyApp". constructors*. apply* ok_type_strengthening. } *)
+    (* Qed. *)
 
-    Lemma ok_data_tvar_strengthening :
-      forall G1 G2 x k d,
-        ok_data (G1 & x ~ BindTVar k & G2) d ->
-        ok_data (G1 & G2) d.
-    Proof.
-      introv Hd. unfolds ok_data.
-      splits*. introv Hbind.
-      lets [Hbind' Hk]: (proj2 Hd) Hbind.
-      splits.
-      - binds_cases Hbind' ; auto.
-      - introv Hkin. lets [ ? (? & Hbindk) ] : Hk Hkin.
-        binds_cases Hbindk ; eauto.
-    Qed.
+    (* Lemma ok_type_lct : *)
+    (*   forall Gamma T k, *)
+    (*     Gamma |= T ~:: k -> *)
+    (*     lct T. *)
+    (* Proof. introv Hk ; induction* Hk. Qed. *)
+    (* #[export] *)
+    (*  Hint Resolve ok_type_lct : mcore. *)
 
-    Lemma ok_data_bsubst :
-      forall G1 G2 X T d,
-        ok_data (G1 & G2) d ->
-        ok_data (G1 & map (bsubst X T) G2) d.
-    Proof.
-      introv Hd. unfolds ok_data.
-      splits*. introv Hbind.
-      lets [Hbind' Hk]: (proj2 Hd) Hbind.
-      splits.
-      - binds_cases Hbind' ; auto.
-        replaces BindTName with (bsubst X T BindTName) ; auto.
-      - introv Hkin. lets [ d' (ty & Hbindk) ] : Hk Hkin.
-        binds_cases Hbindk ; eauto.
-        exists d' ({X => T} ty).
-        replaces (BindCon d' ({X => T} ty) T0) with (bsubst X T (BindCon d' ty T0)) ; auto.
-    Qed.
+    (* (* Lemma ok_ctx_concat_inv : forall G2 G1, ok_ctx (G1 ++ G2) -> ok_ctx G1. *) *)
+    (* (* Proof. *) *)
+    (* (*   induction G2 ; intros. *) *)
+    (* (*   - rew_list in H. apply H. *) *)
+    (* (*   - specializes IHG2 (G1 & a). rew_list in *. *) *)
+    (* (*     apply IHG2 in H. inverts* H. *) *)
+    (* (*     + false. apply* nil_eq_last_inv. *) *)
+    (* (*     + lets . *) *)
+    (* (*       rew_list in H1. *) *)
+    (* (*     inverts H1. *) *)
+    (* (*   introv Hok. *) *)
 
-    Lemma ok_kind_tvar_strengthening :
-      forall G1 G2 x k' k,
-        ok_kind (G1 & x ~ BindTVar k' & G2) k ->
-        ok_kind (G1 & G2) k.
-    Proof. introv Hk. induction* Hk. Qed.
+    (* Lemma ok_kind_weakening : *)
+    (*   forall G2 G1 b k, *)
+    (*     ok_kind (G1 ++ G2) k -> *)
+    (*     ok_kind (G1 & b ++ G2) k. *)
+    (* Proof. introv Hk. induction* Hk. Qed. *)
 
-    Lemma ok_kind_bsubst :
-      forall G1 G2 X T k,
-        ok_kind (G1 & G2) k ->
-        ok_kind (G1 & map (bsubst X T) G2) k.
-    Proof. introv Hk. induction* Hk. Qed.
+    (* Lemma ok_type_tname_weakening : *)
+    (*   forall G2 G1 T k, *)
+    (*     (G1 ++ G2) |= T ~:: k -> *)
+    (*     (G1 & BindTName ++ G2) |= T ~:: k. *)
+    (* Proof. *)
+    (*   introv Hk. *)
+    (*   remember (G1 ++ G2) as Gamma. gen G2. *)
+    (*   induction* Hk; intros; substs. *)
+    (*   { Case "TyFVar". constructors*. constructors. apply* binds_weaken. } *)
+    (*   { Case "TyAll". apply_fresh* KAll. apply* ok_kind_weakening. *)
+    (*     apply_ih_bind* H1. *)
+    (*     constructor*. apply* ok_kind_weakening. } *)
+    (* Qed. *)
 
-    Lemma ok_type_tsubst :
-      forall G1 G2 X T1 T2 k k',
-        G1 & X ~ BindTVar k' & G2 |= T1 ~:: k ->
-        G1 |= T2 ~:: k' ->
-        ok_ctx (G1 & map (bsubst X T2) G2) ->
-        G1 & map (bsubst X T2) G2 |= {X => T2} T1 ~:: k.
-    Proof with eauto with mcore.
-      introv Hkt1 Hkt2 Hctx.
-      remember (G1 & X ~ BindTVar k' & G2) as G. gen G2.
-      induction Hkt1; intros; substs; simpls*.
-      { Case "TyFVar". solve_var.
-        + binds_get H0. lets* [Hok ?] : ok_concat_inv (ok_ctx_ok _ Hctx).
-          apply_empty* ok_type_weakening.
-        + binds_cases H0...
-          constructors*. apply binds_concat_right.
-          replaces (BindTVar k) with (bsubst X T2 (BindTVar k))... }
-      { Case "TyAll". assert (Hk : ok_kind (G1 & map (bsubst X T2) G2) k).
-        apply* ok_kind_bsubst. apply* ok_kind_tvar_strengthening.
-        apply_fresh* KAll.
-        assert (lct T2) by apply* ok_type_lct.
-        rewrite~ tsubst_topen_comm.
-        replaces (G1 & map (bsubst X T2) G2 & y ~ BindTVar k)
-          with (G1 & map (bsubst X T2) (G2 & y ~ BindTVar k))...
-        + autorewrite with rew_ctx_map rew_ctx_concat ; auto.
-        + apply~ H1.
-          * autorewrite with rew_ctx_concat ; auto.
-          * autorewrite with rew_ctx_map rew_ctx_concat... }
-    Qed.
+    (* Lemma ok_ctx_ok_type : *)
+    (*   forall Gamma x T, *)
+    (*     ok_ctx Gamma -> *)
+    (*     var_in x T Gamma -> *)
+    (*     Gamma |= T ~:: KiType. *)
+    (* Proof. *)
+    (*   introv Hctx Hbind. *)
+    (*   induction* Hctx ; unfolds var_in ; rew_ctx in *. (* ; try (binds_cases Hbind ; apply_empty* ok_type_weakening). *) *)
+    (*   { Case "CtxEmpty". inverts Hbind. } *)
+    (*   { Case "CtxTName". apply* ok_type_weakening. *)
+    (*     lets Hwot : (Nth_last_inv x _ Hbind). *)
+    (*     inverts* EQ. } *)
+    (*   { Case "CtxVar". inverts* EQ. } *)
+    (* Qed. *)
 
-    Lemma bsubst_ok_ctx :
-      forall G1 G2 X T2 k,
-        G1 |= T2 ~:: k ->
-        ok_ctx (G1 & X ~ BindTVar k & G2) ->
-        ok_ctx (G1 & map (bsubst X T2) G2).
-    Proof.
-      introv Htk Hctx.
-      induction G2 using ctx_ind.
-      { Case "Empty". autorewrite with rew_ctx_map rew_ctx_concat in *.
-        apply* ok_ctx_push. }
-      { Case "Push". autorewrite with rew_ctx_map rew_ctx_concat in *.
-        specializes IHG2 (ok_ctx_push _ _ _ Hctx).
-        lets [? Hdisj] : ok_push_inv (ok_ctx_ok _ Hctx).
-        destruct v.
-        { SCase "BindTName". constructor~. }
-        { SCase "BindCon". forwards (Hd & Htk' & HT): ok_ctx_con_inv Hctx.
-          constructor~.
-          - applys ok_data_bsubst. apply* ok_data_tvar_strengthening.
-          - applys* ok_type_tsubst Htk.
-          - binds_cases HT ; auto.
-            replaces BindTName with (bsubst X T2 BindTName) ; auto. }
-        { SCase "BindTVar". forwards Hk: ok_ctx_tvar_inv Hctx.
-          constructor~. applys ok_kind_bsubst. apply* ok_kind_tvar_strengthening. }
-        { SCase "BindVar". forwards Htk': ok_ctx_var_inv Hctx.
-          constructor~. applys* ok_type_tsubst Htk'. }
-        { SCase "BindMatch". constructor~. } }
-    Qed.
 
-    Lemma ok_ctx_concat :
-      forall G1 G2,
-        ok_ctx (G1 & G2) ->
-        ok_ctx G1.
-    Proof with eauto.
-      introv Hctx.
-      induction G2 using ctx_ind.
-      { Case "Empty". rew_ctx_concat in *... }
-      { Case "Push". apply IHG2. rew_ctx_concat in *.
-        apply* ok_ctx_push. }
-    Qed.
+    (* Lemma ok_term_lct : *)
+    (*   forall Gamma t T, *)
+    (*     Gamma |= t ~: T -> *)
+    (*     lct T. *)
+    (* Proof with eauto using ok_type_lct. *)
+    (*   introv hasType. *)
+    (*   induction* hasType ; simple_math... *)
+    (*   { Case "TmLam". constructors... *)
+    (*     pick_fresh_gen L y... } *)
+    (*   { Case "TmApp". inverts* IHhasType1. } *)
+    (*   { Case "TmTyLam". inverts* IHhasType. *)
+    (*     assert(Hlct: lct ty2)... *)
+    (*     pick_fresh X. rewrite *(@tsubst_intro X). *)
+    (*     apply* tsubst_lct. } *)
+    (* Qed. *)
+    (* #[export] *)
+    (*  Hint Resolve ok_term_lct : mcore. *)
 
-    Lemma ok_type_notin :
-      forall Gamma T k X,
-        Gamma |= T ~:: k ->
-        X # Gamma ->
-        X \notin ftv T.
-    Proof.
-      introv Htk Hfresh.
-      induction Htk; simpls*.
-      { Case "TyFVar". intros contra.
-        rewrite in_singleton in contra. substs.
-        apply get_none in Hfresh.
-        apply binds_get in H0.
-        fequals. }
-      { Case "TyAll". pick_fresh Y.
-        forwards~ Hnin: H0 Y.
-        applys~ topen_notin Y. }
-    Qed.
+    (* Lemma ok_term_lc : *)
+    (*   forall Gamma t T, *)
+    (*     Gamma |= t ~: T -> *)
+    (*     lc t. *)
+    (* Proof with eauto using ok_term_lct, ok_type_lct with mcore. *)
+    (*   introv Htype. *)
+    (*   induction* Htype; intros. *)
+    (* Qed. *)
+    (* #[export] *)
+    (*  Hint Resolve ok_term_lc : mcore. *)
 
-    Lemma ctx_bsubst_fresh :
-      forall Gamma X T2,
-        ok_ctx Gamma ->
-        X # Gamma ->
-        Gamma = map (bsubst X T2) Gamma.
-    Proof with eauto using ok_ctx_push.
-      introv Hctx Hfresh.
-      induction Gamma using ctx_ind.
-      { Case "Empty". rewrite~ map_empty. }
-      { Case "Push". autorewrite with rew_ctx_map.
-        rewrite <- IHGamma...
-        destruct~ v ; repeat fequals ; unfold bsubst ; rewrite* tsubst_fresh.
-        { SCase "BindCon".
-          apply ok_ctx_con_inv in Hctx as (? & Hkt & ?).
-          apply* ok_type_notin. }
-        { SCase "BindVar".
-          apply ok_ctx_var_inv in Hctx.
-          apply* ok_type_notin. } }
-    Qed.
+    (* Lemma ok_ctx_push : *)
+    (*   forall G1 x b, *)
+    (*     ok_ctx (G1 & x ~ b) -> *)
+    (*     ok_ctx G1. *)
+    (* Proof. *)
+    (*   introv Hwf. *)
+    (*   inverts Hwf ; try (apply eq_push_inv in H; inverts H as []; substs*. *)
+    (*   false. apply *empty_push_inv. *)
+    (* Qed. *)
 
-    Lemma ok_term_tsubst :
-      forall G2 G1 t k T1 T2 X,
-        G1 & X ~ BindTVar k & G2 |= t ~: T1 ->
-        G1 |= T2 ~:: k ->
-        G1 & map (bsubst X T2) G2 |= [{X => T2}]t ~: ({X => T2}T1).
-    Proof with eauto using ok_ctx_strengthening, bsubst_ok_ctx with mcore.
-      introv hasType Hctx.
-      remember (G1 & X ~ BindTVar k & G2) as G. gen G2.
-      induction hasType; intros; simpls; substs...
-      { Case "TmFVar".
-        binds_cases H0 ; constructors ;
-          replaces (BindVar ({X => T2} ty)) with (bsubst X T2 (BindVar ty))...
-        apply ok_ctx_concat in H.
-        assert (X # G1) by apply* ok_push_inv.
-        rewrite* (@ctx_bsubst_fresh G1 X T2). }
-      { Case "TmLam". apply_fresh* TLam as x.
-        + apply* ok_type_tsubst. apply* bsubst_ok_ctx.
-        + rewrite tsubst_t_open_comm.
-          replaces (G1 & map (bsubst X T2) G2 & x ~ BindVar ({X => T2}ty1))
-            with (G1 & map (bsubst X T2) (G2 & x ~ BindVar ty1)).
-          autorewrite with rew_ctx_map rew_ctx_concat ; auto.
-          apply~ H1. rewrite~ concat_assoc. }
-      { Case "TmTyLam". apply_fresh* TTyLam.
-        + apply ok_kind_bsubst. apply* ok_kind_tvar_strengthening.
-        + replaces (G1 & map (bsubst X T2) G2 & y ~ BindTVar k0)
-            with (G1 & map (bsubst X T2) (G2 & y ~ BindTVar k0)).
-          autorewrite with rew_env_map rew_env_concat ; auto.
-          rewrite~ tsubst_topen_comm...
-          rewrite topen_t_tsubst_comm...
-          apply~ H1. rewrite~ concat_assoc. }
-      { Case "TmTyApp".
-        rewrite tsubst_topen_distr... constructors*.
-        apply* ok_type_tsubst. }
-    Qed.
+    (* Lemma ok_type_ok_ctx : *)
+    (*   forall Gamma T k, *)
+    (*     Gamma |= T ~:: k -> *)
+    (*     ok_ctx Gamma. *)
+    (* Proof. *)
+    (*   introv hasType. *)
+    (*   induction* hasType; pick_fresh_gen L x; *)
+    (*     eauto using ok_ctx_push. *)
+    (* Qed. *)
+    (* #[export] *)
+    (*  Hint Resolve ok_type_ok_ctx : mcore. *)
+
+    (* Lemma ok_term_ok_ctx : *)
+    (*   forall Gamma t T, *)
+    (*     Gamma |= t ~: T -> *)
+    (*     ok_ctx Gamma. *)
+    (* Proof. *)
+    (*   introv hasType. *)
+    (*   induction* hasType; pick_fresh_gen L x; *)
+    (*     eauto using ok_ctx_push. *)
+    (* Qed. *)
+    (* #[export] *)
+    (*  Hint Resolve ok_term_ok_ctx : mcore. *)
+
+    (* Lemma ok_term_weakening : *)
+    (*   forall G3 G2 G1 t T, *)
+    (*     G1 & G3 |= t ~: T -> *)
+    (*     ok_ctx (G1 & G2 & G3) -> *)
+    (*     G1 & G2 & G3 |= t ~: T. *)
+    (* Proof. *)
+    (*   introv hasType Hctx. remember (G1 & G3) as H. gen G3. *)
+    (*   induction hasType; intros; substs*. *)
+    (*   { Case "TmFVar". constructors*. apply* binds_weaken. } *)
+    (*   { Case "TmLam". apply_fresh* TLam as y. *)
+    (*     - apply* ok_type_weakening. *)
+    (*     - apply_ih_bind* H1. *)
+    (*       constructors*. *)
+    (*       apply* ok_type_weakening. } *)
+    (*   { Case "TmTyLam". apply_fresh* TTyLam as X. *)
+    (*     - apply* ok_kind_weakening. *)
+    (*     - apply_ih_bind* H1. constructors*. apply* ok_kind_weakening. } *)
+    (*   { Case "TmTyApp". constructors*. apply* ok_type_weakening. } *)
+    (* Qed. *)
+
+    (* Lemma ok_data_strengthening : *)
+    (*   forall G1 G2 x T d, *)
+    (*     ok_data (G1 & x ~ BindVar T & G2) d -> *)
+    (*     ok_data (G1 & G2) d. *)
+    (* Proof. *)
+    (*   introv Hd. unfolds ok_data. *)
+    (*   splits*. introv Hbind. *)
+    (*   lets [Hbind' Hk]: (proj2 Hd) Hbind. *)
+    (*   splits. *)
+    (*   - binds_cases Hbind' ; auto. *)
+    (*   - introv Hkin. lets [ ? (? & Hbindk) ] : Hk Hkin. *)
+    (*     binds_cases Hbindk ; eauto. *)
+    (* Qed. *)
+
+    (* Lemma ok_kind_strengthening : *)
+    (*   forall G1 G2 x T k, *)
+    (*     ok_kind (G1 & x ~ BindVar T & G2) k -> *)
+    (*     ok_kind (G1 & G2) k. *)
+    (* Proof. introv Hk. induction* Hk. Qed. *)
+
+    (* Lemma ok_type_strengthening : *)
+    (*   forall G1 G2 x T1 T2 k, *)
+    (*     G1 & x ~ BindVar T2 & G2 |= T1 ~:: k -> *)
+    (*     ok_ctx (G1 & G2) -> *)
+    (*     G1 & G2 |= T1 ~:: k. *)
+    (* Proof. *)
+    (*   introv Htk. remember (G1 & x ~ BindVar T2 & G2) as G. gen G2. *)
+    (*   induction Htk; intros; substs*. *)
+    (*   { Case "TyFVar". constructors*. *)
+    (*     binds_cases H0 ; auto. } *)
+    (*   { Case "TyAll". apply_fresh* KAll as X. *)
+    (*     apply* ok_kind_strengthening. *)
+    (*     apply_ih_bind* H1. constructor*. apply* ok_kind_strengthening. } *)
+    (* Qed. *)
+
+    (* Lemma ok_ctx_con_inv : *)
+    (*   forall Gamma K d ty T, *)
+    (*     ok_ctx (Gamma & K ~ BindCon d ty T) -> *)
+    (*     ok_data Gamma d /\ Gamma |= ty ~:: KiType /\ binds T BindTName Gamma. *)
+    (* Proof. *)
+    (*   introv Hctx. *)
+    (*   inverts Hctx ; try (apply eq_push_inv in H as (? & ? & ?); substs* ; splits* ; fequals). *)
+    (*   false. apply* empty_push_inv. *)
+    (* Qed. *)
+
+    (* Lemma ok_ctx_tvar_inv : *)
+    (*   forall Gamma X k, *)
+    (*     ok_ctx (Gamma & X ~ BindTVar k) -> *)
+    (*     ok_kind Gamma k. *)
+    (* Proof. *)
+    (*   introv Hctx. *)
+    (*   inverts Hctx ; try (apply eq_push_inv in H as (? & ? & ?); substs* ; fequals). *)
+    (*   false. apply* empty_push_inv. *)
+    (* Qed. *)
+
+    (* Lemma ok_ctx_var_inv : *)
+    (*   forall Gamma x T, *)
+    (*     ok_ctx (Gamma & x ~ BindVar T) -> *)
+    (*     Gamma |= T ~:: KiType. *)
+    (* Proof. *)
+    (*   introv Hctx. *)
+    (*   inverts Hctx ; try (apply eq_push_inv in H as (? & ? & ?); substs* ; fequals). *)
+    (*   false. apply* empty_push_inv. *)
+    (* Qed. *)
+
+    (* Lemma ok_ctx_strengthening : *)
+    (*   forall G1 x T G3, *)
+    (*     ok_ctx (G1 & x ~ BindVar T & G3) -> *)
+    (*     ok_ctx (G1 & G3). *)
+    (* Proof. *)
+    (*   introv Hctx. induction G3 using ctx_ind. *)
+    (*   { Case "Empty". rewrite concat_empty_r in *. apply* ok_ctx_push. } *)
+    (*   { Case "Push". rewrite concat_assoc in *. *)
+    (*     specializes IHG3 (ok_ctx_push _ _ _ Hctx). *)
+    (*     lets [? Hdisj] : ok_push_inv (ok_ctx_ok _ Hctx). *)
+    (*     destruct v. *)
+    (*     { SCase "BindTName". constructor~. } *)
+    (*     { SCase "BindCon". forwards [ Hd (Htk & HT)]: ok_ctx_con_inv Hctx. *)
+    (*       constructor~. *)
+    (*       - applys ok_data_strengthening Hd. *)
+    (*       - applys* ok_type_strengthening Htk. *)
+    (*       - binds_cases HT ; auto. } *)
+    (*     { SCase "BindTVar". forwards Hk: ok_ctx_tvar_inv Hctx. *)
+    (*       constructor~. applys ok_kind_strengthening Hk. } *)
+    (*     { SCase "BindVar". forwards Htk: ok_ctx_var_inv Hctx. *)
+    (*       constructor~. applys* ok_type_strengthening Htk. } *)
+    (*     { SCase "BindMatch". constructor~. } } *)
+    (* Qed. *)
+
+    (* Lemma ok_term_subst : *)
+    (*   forall G2 G1 x T1 T2 t1 t2, *)
+    (*     G1 & x ~ BindVar T2 & G2 |= t1 ~: T1 -> *)
+    (*     G1 |= t2 ~: T2 -> *)
+    (*     G1 & G2 |= [x => t2]t1 ~: T1. *)
+    (* Proof with eauto using ok_term_lc, ok_ctx_strengthening, ok_type_strengthening with mcore. *)
+    (*   introv hasType1 hasType2. *)
+    (*   remember (G1 & x ~ BindVar T2 & G2) as G. gen G2. *)
+    (*   induction hasType1; intros; simpls; substs... *)
+    (*   { Case "TmFVar". solve_var. *)
+    (*     - binds_get H0... apply_empty ok_term_weakening... *)
+    (*     - binds_cases H0... } *)
+    (*   { Case "TmLam". apply_fresh* TLam as y... *)
+    (*     rewrite subst_open_comm... apply_ih_bind* H1. } *)
+    (*   { Case "TmTyLam". apply_fresh* TTyLam as X. apply* ok_kind_strengthening. *)
+    (*     rewrite* topen_t_subst_comm. apply_ih_bind* H1. } *)
+    (*   { Case "TmTyApp". constructors*. apply* ok_type_strengthening. } *)
+    (* Qed. *)
+
+    (* Lemma ok_data_tvar_strengthening : *)
+    (*   forall G1 G2 x k d, *)
+    (*     ok_data (G1 & x ~ BindTVar k & G2) d -> *)
+    (*     ok_data (G1 & G2) d. *)
+    (* Proof. *)
+    (*   introv Hd. unfolds ok_data. *)
+    (*   splits*. introv Hbind. *)
+    (*   lets [Hbind' Hk]: (proj2 Hd) Hbind. *)
+    (*   splits. *)
+    (*   - binds_cases Hbind' ; auto. *)
+    (*   - introv Hkin. lets [ ? (? & Hbindk) ] : Hk Hkin. *)
+    (*     binds_cases Hbindk ; eauto. *)
+    (* Qed. *)
+
+    (* Lemma ok_data_bsubst : *)
+    (*   forall G1 G2 X T d, *)
+    (*     ok_data (G1 & G2) d -> *)
+    (*     ok_data (G1 & map (bsubst X T) G2) d. *)
+    (* Proof. *)
+    (*   introv Hd. unfolds ok_data. *)
+    (*   splits*. introv Hbind. *)
+    (*   lets [Hbind' Hk]: (proj2 Hd) Hbind. *)
+    (*   splits. *)
+    (*   - binds_cases Hbind' ; auto. *)
+    (*     replaces BindTName with (bsubst X T BindTName) ; auto. *)
+    (*   - introv Hkin. lets [ d' (ty & Hbindk) ] : Hk Hkin. *)
+    (*     binds_cases Hbindk ; eauto. *)
+    (*     exists d' ({X => T} ty). *)
+    (*     replaces (BindCon d' ({X => T} ty) T0) with (bsubst X T (BindCon d' ty T0)) ; auto. *)
+    (* Qed. *)
+
+    (* Lemma ok_kind_tvar_strengthening : *)
+    (*   forall G1 G2 x k' k, *)
+    (*     ok_kind (G1 & x ~ BindTVar k' & G2) k -> *)
+    (*     ok_kind (G1 & G2) k. *)
+    (* Proof. introv Hk. induction* Hk. Qed. *)
+
+    (* Lemma ok_kind_bsubst : *)
+    (*   forall G1 G2 X T k, *)
+    (*     ok_kind (G1 & G2) k -> *)
+    (*     ok_kind (G1 & map (bsubst X T) G2) k. *)
+    (* Proof. introv Hk. induction* Hk. Qed. *)
+
+    (* Lemma ok_type_tsubst : *)
+    (*   forall G1 G2 X T1 T2 k k', *)
+    (*     G1 & X ~ BindTVar k' & G2 |= T1 ~:: k -> *)
+    (*     G1 |= T2 ~:: k' -> *)
+    (*     ok_ctx (G1 & map (bsubst X T2) G2) -> *)
+    (*     G1 & map (bsubst X T2) G2 |= {X => T2} T1 ~:: k. *)
+    (* Proof with eauto with mcore. *)
+    (*   introv Hkt1 Hkt2 Hctx. *)
+    (*   remember (G1 & X ~ BindTVar k' & G2) as G. gen G2. *)
+    (*   induction Hkt1; intros; substs; simpls*. *)
+    (*   { Case "TyFVar". solve_var. *)
+    (*     + binds_get H0. lets* [Hok ?] : ok_concat_inv (ok_ctx_ok _ Hctx). *)
+    (*       apply_empty* ok_type_weakening. *)
+    (*     + binds_cases H0... *)
+    (*       constructors*. apply binds_concat_right. *)
+    (*       replaces (BindTVar k) with (bsubst X T2 (BindTVar k))... } *)
+    (*   { Case "TyAll". assert (Hk : ok_kind (G1 & map (bsubst X T2) G2) k). *)
+    (*     apply* ok_kind_bsubst. apply* ok_kind_tvar_strengthening. *)
+    (*     apply_fresh* KAll. *)
+    (*     assert (lct T2) by apply* ok_type_lct. *)
+    (*     rewrite~ tsubst_topen_comm. *)
+    (*     replaces (G1 & map (bsubst X T2) G2 & y ~ BindTVar k) *)
+    (*       with (G1 & map (bsubst X T2) (G2 & y ~ BindTVar k))... *)
+    (*     + autorewrite with rew_ctx_map rew_ctx_concat ; auto. *)
+    (*     + apply~ H1. *)
+    (*       * autorewrite with rew_ctx_concat ; auto. *)
+    (*       * autorewrite with rew_ctx_map rew_ctx_concat... } *)
+    (* Qed. *)
+
+    (* Lemma bsubst_ok_ctx : *)
+    (*   forall G1 G2 X T2 k, *)
+    (*     G1 |= T2 ~:: k -> *)
+    (*     ok_ctx (G1 & X ~ BindTVar k & G2) -> *)
+    (*     ok_ctx (G1 & map (bsubst X T2) G2). *)
+    (* Proof. *)
+    (*   introv Htk Hctx. *)
+    (*   induction G2 using ctx_ind. *)
+    (*   { Case "Empty". autorewrite with rew_ctx_map rew_ctx_concat in *. *)
+    (*     apply* ok_ctx_push. } *)
+    (*   { Case "Push". autorewrite with rew_ctx_map rew_ctx_concat in *. *)
+    (*     specializes IHG2 (ok_ctx_push _ _ _ Hctx). *)
+    (*     lets [? Hdisj] : ok_push_inv (ok_ctx_ok _ Hctx). *)
+    (*     destruct v. *)
+    (*     { SCase "BindTName". constructor~. } *)
+    (*     { SCase "BindCon". forwards (Hd & Htk' & HT): ok_ctx_con_inv Hctx. *)
+    (*       constructor~. *)
+    (*       - applys ok_data_bsubst. apply* ok_data_tvar_strengthening. *)
+    (*       - applys* ok_type_tsubst Htk. *)
+    (*       - binds_cases HT ; auto. *)
+    (*         replaces BindTName with (bsubst X T2 BindTName) ; auto. } *)
+    (*     { SCase "BindTVar". forwards Hk: ok_ctx_tvar_inv Hctx. *)
+    (*       constructor~. applys ok_kind_bsubst. apply* ok_kind_tvar_strengthening. } *)
+    (*     { SCase "BindVar". forwards Htk': ok_ctx_var_inv Hctx. *)
+    (*       constructor~. applys* ok_type_tsubst Htk'. } *)
+    (*     { SCase "BindMatch". constructor~. } } *)
+    (* Qed. *)
+
+    (* Lemma ok_ctx_concat : *)
+    (*   forall G1 G2, *)
+    (*     ok_ctx (G1 & G2) -> *)
+    (*     ok_ctx G1. *)
+    (* Proof with eauto. *)
+    (*   introv Hctx. *)
+    (*   induction G2 using ctx_ind. *)
+    (*   { Case "Empty". rew_ctx_concat in *... } *)
+    (*   { Case "Push". apply IHG2. rew_ctx_concat in *. *)
+    (*     apply* ok_ctx_push. } *)
+    (* Qed. *)
+
+    (* Lemma ok_type_notin : *)
+    (*   forall Gamma T k X, *)
+    (*     Gamma |= T ~:: k -> *)
+    (*     X # Gamma -> *)
+    (*     X \notin ftv T. *)
+    (* Proof. *)
+    (*   introv Htk Hfresh. *)
+    (*   induction Htk; simpls*. *)
+    (*   { Case "TyFVar". intros contra. *)
+    (*     rewrite in_singleton in contra. substs. *)
+    (*     apply get_none in Hfresh. *)
+    (*     apply binds_get in H0. *)
+    (*     fequals. } *)
+    (*   { Case "TyAll". pick_fresh Y. *)
+    (*     forwards~ Hnin: H0 Y. *)
+    (*     applys~ topen_notin Y. } *)
+    (* Qed. *)
+
+    (* Lemma ctx_bsubst_fresh : *)
+    (*   forall Gamma X T2, *)
+    (*     ok_ctx Gamma -> *)
+    (*     X # Gamma -> *)
+    (*     Gamma = map (bsubst X T2) Gamma. *)
+    (* Proof with eauto using ok_ctx_push. *)
+    (*   introv Hctx Hfresh. *)
+    (*   induction Gamma using ctx_ind. *)
+    (*   { Case "Empty". rewrite~ map_empty. } *)
+    (*   { Case "Push". autorewrite with rew_ctx_map. *)
+    (*     rewrite <- IHGamma... *)
+    (*     destruct~ v ; repeat fequals ; unfold bsubst ; rewrite* tsubst_fresh. *)
+    (*     { SCase "BindCon". *)
+    (*       apply ok_ctx_con_inv in Hctx as (? & Hkt & ?). *)
+    (*       apply* ok_type_notin. } *)
+    (*     { SCase "BindVar". *)
+    (*       apply ok_ctx_var_inv in Hctx. *)
+    (*       apply* ok_type_notin. } } *)
+    (* Qed. *)
+
+    (* Lemma ok_term_tsubst : *)
+    (*   forall G2 G1 t k T1 T2 X, *)
+    (*     G1 & X ~ BindTVar k & G2 |= t ~: T1 -> *)
+    (*     G1 |= T2 ~:: k -> *)
+    (*     G1 & map (bsubst X T2) G2 |= [{X => T2}]t ~: ({X => T2}T1). *)
+    (* Proof with eauto using ok_ctx_strengthening, bsubst_ok_ctx with mcore. *)
+    (*   introv hasType Hctx. *)
+    (*   remember (G1 & X ~ BindTVar k & G2) as G. gen G2. *)
+    (*   induction hasType; intros; simpls; substs... *)
+    (*   { Case "TmFVar". *)
+    (*     binds_cases H0 ; constructors ; *)
+    (*       replaces (BindVar ({X => T2} ty)) with (bsubst X T2 (BindVar ty))... *)
+    (*     apply ok_ctx_concat in H. *)
+    (*     assert (X # G1) by apply* ok_push_inv. *)
+    (*     rewrite* (@ctx_bsubst_fresh G1 X T2). } *)
+    (*   { Case "TmLam". apply_fresh* TLam as x. *)
+    (*     + apply* ok_type_tsubst. apply* bsubst_ok_ctx. *)
+    (*     + rewrite tsubst_t_open_comm. *)
+    (*       replaces (G1 & map (bsubst X T2) G2 & x ~ BindVar ({X => T2}ty1)) *)
+    (*         with (G1 & map (bsubst X T2) (G2 & x ~ BindVar ty1)). *)
+    (*       autorewrite with rew_ctx_map rew_ctx_concat ; auto. *)
+    (*       apply~ H1. rewrite~ concat_assoc. } *)
+    (*   { Case "TmTyLam". apply_fresh* TTyLam. *)
+    (*     + apply ok_kind_bsubst. apply* ok_kind_tvar_strengthening. *)
+    (*     + replaces (G1 & map (bsubst X T2) G2 & y ~ BindTVar k0) *)
+    (*         with (G1 & map (bsubst X T2) (G2 & y ~ BindTVar k0)). *)
+    (*       autorewrite with rew_env_map rew_env_concat ; auto. *)
+    (*       rewrite~ tsubst_topen_comm... *)
+    (*       rewrite topen_t_tsubst_comm... *)
+    (*       apply~ H1. rewrite~ concat_assoc. } *)
+    (*   { Case "TmTyApp". *)
+    (*     rewrite tsubst_topen_distr... constructors*. *)
+    (*     apply* ok_type_tsubst. } *)
+    (* Qed. *)
 
   End Typing.
 End Typing.
